Remove wordp specializations

markov/bin2unary.lisp
@@ -3,102 +3,6 @@
 (local (include-book "std/basic/inductions" :dir :system))
 (local (include-book "arithmetic/top" :dir :system))
 
-(defund word-01-p (x)
-  (declare (xargs :guard t))
-  (wordp x '(#\0 #\1)))
-
-(defrule |word-01-p is true-listp|
-  (implies (word-01-p x) (true-listp x))
-  :enable word-01-p)
-
-(defruled |nth word-01-p is member|
-  (implies
-    (and (word-01-p inp)
-         (natp i)
-         (< i (len inp)))
-    (member (nth i inp) '(#\0 #\1)))
-  :enable word-01-p)
-
-(defrule |take word-01-p|
-  (implies (and (word-01-p x)
-                (<= n (len x)))
-           (word-01-p (take n x)))
-  :enable word-01-p)
-
-(defrule |nthcdr word-01-p|
-  (implies (word-01-p x)
-           (word-01-p (nthcdr n x)))
-  :enable word-01-p)
-
-(defrule listpos-append-word-01-p
-  (implies
-    (and
-      (word-01-p x)
-      (consp pat)
-      (not (member (car pat) '(#\0 #\1))))
-    (equal (listpos pat (append x y))
-           (and (listpos pat y)
-                (+ (len x) (listpos pat y)))))
-  :enable word-01-p)
-
-(defrule sublistp-append-word-01-p
-  (implies
-    (and
-      (word-01-p x)
-      (not (member (car pat) '(#\0 #\1))))
-    (equal (sublistp pat (append x y))
-           (sublistp pat y)))
-  :enable word-01-p)
-
-(defund word-0bar-p (x)
-  (declare (xargs :guard t))
-  (wordp x '(#\0 #\|)))
-
-(defrule |word-0bar-p is true-listp|
-  (implies (word-0bar-p x) (true-listp x))
-  :enable word-0bar-p)
-
-(defruled |nth word-0bar-p is member|
-  (implies
-    (and (word-0bar-p inp)
-         (natp i)
-         (< i (len inp)))
-    (member (nth i inp) '(#\0 #\|)))
-  :enable word-0bar-p)
-
-(defrule |take word-0bar-p|
-  (implies (and (word-0bar-p x)
-                (<= n (len x)))
-           (word-0bar-p (take n x)))
-  :enable word-0bar-p)
-
-(defrule |nthcdr word-0bar-p|
-  (implies (word-0bar-p x)
-           (word-0bar-p (nthcdr n x)))
-  :enable word-0bar-p)
-
-(defrule listpos-append-word-0bar-p
-  (implies
-    (and
-      (word-0bar-p x)
-      (consp pat)
-      (not (member (car pat) '(#\0 #\|))))
-    (equal (listpos pat (append x y))
-           (and (listpos pat y)
-                (+ (len x) (listpos pat y)))))
-  :enable word-0bar-p)
-
-(defrule sublistp-append-word-0bar-p
-  (implies
-    (and
-      (word-0bar-p x)
-      (not (member (car pat) '(#\0 #\|))))
-    (equal (sublistp pat (append x y))
-           (sublistp pat y)))
-  :enable word-0bar-p)
-
-;------------------------------------
-
 (defconst *scheme-bin2unary-en*
   (list
     (mks->  "|0" "0||")
@@ -117,10 +21,10 @@
         ((eql (car x) #\1) (list* #\0 #\| (replace-ones (cdr x))))
         (t (list* (car x) (replace-ones (cdr x))))))
 
-(defruled |word-0bar-p replace-ones|
-  (implies (word-01-p x)
-           (word-0bar-p (replace-ones x)))
-  :enable (replace-ones word-0bar-p word-01-p)
+(defruled |wordp replace-ones 0bar|
+  (implies (wordp x '(#\0 #\1))
+           (wordp (replace-ones x) '(#\0 #\|)))
+  :enable replace-ones
   :induct (len x))
 
 (defrule |replace-ones append|
@@ -130,7 +34,7 @@
   :induct (len x))
 
 (defund step1 (inp n)
-  (declare (xargs :guard (and (word-01-p inp) (natp n))))
+  (declare (xargs :guard (and (wordp inp'(#\0 #\1)) (natp n))))
   (append (replace-ones (take n inp)) (nthcdr n inp)))
 
 (defrule |step1 0|
@@ -139,7 +43,7 @@
 
 (defrule |step1 len|
   (implies
-    (word-01-p inp)
+    (wordp inp'(#\0 #\1))
     (equal (step1 inp (len inp))
            (replace-ones inp)))
   :enable step1)
@@ -147,7 +51,7 @@
 (defrule |step1 same when #\0|
   (implies
     (and
-      (word-01-p inp)
+      (wordp inp'(#\0 #\1))
       (natp n)
       (< n (len inp))
       (eql (nth n inp) #\0))
@@ -158,14 +62,14 @@
 (defruled |step1 applicable when #\1|
   (implies
     (and
-      (word-01-p inp)
+      (wordp inp'(#\0 #\1))
       (natp n)
       (< n (len inp))
       (eql (nth n inp) #\1))
    (equal
       (applicable *scheme-bin2unary-ru* (step1 inp n))
       (mks-> "1" "0|")))
-  :enable (applicable step1 |word-0bar-p replace-ones|)
+  :enable (applicable step1 |wordp replace-ones 0bar|)
   :use (:instance sublistp-append-wordp
          (pat '(#\1))
          (x (replace-ones (take n inp)))
@@ -175,7 +79,7 @@
 (defruled |step1 substp when #\1|
   (implies
     (and
-      (word-01-p inp)
+      (wordp inp '(#\0 #\1))
       (natp n)
       (< n (len inp))
       (eql (nth n inp) #\1))
@@ -183,11 +87,11 @@
   :prep-lemmas (
     (defrule lemma
       (implies
-        (word-0bar-p x)
+        (wordp x '(#\0 #\|))
         (left-wingp x '(#\1)))
-      :enable (word-0bar-p |left-wingp as left-wingp1| left-wingp1)
+      :enable (|left-wingp as left-wingp1| left-wingp1)
       :induct (len x)))
-  :enable (step1 |word-0bar-p replace-ones|
+  :enable (step1 |wordp replace-ones 0bar|
            |take n+1| |nthcdr as cons|)
   :use (:instance substp-lemma
          (x (step1 inp n))
@@ -200,7 +104,7 @@
 (defruled |step1 correct when #\1|
   (implies
     (and
-      (word-01-p inp)
+      (wordp inp '(#\0 #\1))
       (natp n)
       (< n (len inp))
       (eql (nth n inp) #\1))
@@ -213,7 +117,7 @@
 (defruled |step1 correct a|
   (implies
     (and
-      (word-01-p inp)
+      (wordp inp '(#\0 #\1))
       (natp n)
       (< n (len inp)))
     (simple-steps
@@ -222,13 +126,16 @@
       (step1 inp n)
       (step1 inp (1+ n))))
   :enable |step1 correct when #\1|
-  :use (:instance |nth word-01-p is member|
+  :disable |nth wordp is member|
+  :use (:instance |nth wordp is member|
+         (alphabet '(#\0 #\1))
+         (x inp)
          (i n)))
 
 (defruled |step1 correct all|
   (implies
     (and
-      (word-01-p inp)
+      (wordp inp '(#\0 #\1))
       (natp n)
       (<= n (len inp)))
     (simple-steps
@@ -296,32 +203,17 @@
   :rule-classes :linear)
 
 (defund step2 (inp n)
-  (declare (xargs :guard (and (word-01-p inp) (natp n))))
+  (declare (xargs :guard (and (wordp inp '(#\0 #\1)) (natp n))))
   (append (repeat n #\0)
           (repeat (val (take n inp)) #\|)
           (replace-ones (nthcdr n inp))))
-
-(defrule |word-01-p repeat #\0|
-  (word-01-p (repeat n #\0))
-  :enable (word-01-p wordp repeat)
-  :induct (dec-induct n))
-
-(defrule |word-0bar-p repeat #\0|
-  (word-0bar-p (repeat n #\0))
-  :enable (word-0bar-p wordp repeat)
-  :induct (dec-induct n))
-
-(defrule |word-0bar-p repeat bar|
-  (word-0bar-p (repeat n #\|))
-  :enable (word-0bar-p wordp repeat)
-  :induct (dec-induct n))
 
 (defruled |step2 applicable|
   (implies
     (and
       (natp n)
       (posp i)
-      (word-0bar-p y))
+      (wordp y '(#\0 #\|)))
     (equal
       (applicable
         *scheme-bin2unary-ru*
@@ -332,13 +224,14 @@
       (implies
         (and (natp n)
              (posp i)
-             (word-0bar-p y))
+             (wordp y '(#\0 #\|)))
         (not (sublistp '(#\1)
                        (append (repeat n #\0)
                                (repeat i #\|)
                                (cons #\0 y)))))
       :cases ((sublistp '(#\1) y))
-      :hints (("subgoal 1" :use (:instance sublistp-append-word-0bar-p
+      :hints (("subgoal 1" :use (:instance sublistp-append-wordp
+                                  (alphabet '(#\0 #\|))
                                   (pat '(#\1))
                                   (x y)
                                   (y nil)))))
@@ -405,19 +298,15 @@
       (natp n)
       (posp i)
       (natp j)
-      (word-0bar-p y))
+      (wordp y '(#\0 #\|)))
     (simple-stepp
       *scheme-bin2unary-ru*
       (append (repeat n #\0) (repeat i #\|) (list #\0) (repeat j #\|) y)
       (append (repeat n #\0) (repeat (1- i) #\|) (list #\0) (repeat (+ 2 j) #\|) y)))
-  :prep-lemmas (
-    (defrule lemma1
-      (implies
-        (word-0bar-p y)
-        (word-0bar-p (append (repeat j #\|) y)))
-      :enable (word-0bar-p repeat)))
-  :enable (simple-stepp |step2 applicable|)
-  :use |step2 substp|)
+  :enable (simple-stepp wordp-repeat2)
+  :use ((:instance |step2 applicable|
+          (y (append (repeat j #\|) y)))
+        |step2 substp|))
 
 (defruled |step2 correct a|
   (implies
@@ -425,7 +314,7 @@
       (natp n)
       (natp i)
       (natp j)
-      (word-0bar-p y))
+      (wordp y '(#\0 #\|)))
     (simple-steps
       *scheme-bin2unary-ru*
       i
@@ -438,7 +327,7 @@
           (natp n)
           (posp i)
           (natp j)
-          (word-0bar-p y))
+          (wordp y '(#\0 #\|)))
         (simple-steps
           *scheme-bin2unary-ru*
           1
@@ -457,7 +346,7 @@
           (natp i)
           (natp s)
           (<= (* 2 i) s)
-          (word-0bar-p y))
+          (wordp y '(#\0 #\|)))
         (simple-steps
           *scheme-bin2unary-ru*
           i
@@ -480,23 +369,26 @@
 (defrule |val take n+1 inp|
   (implies
     (and
-      (word-01-p inp)
+      (wordp inp '(#\0 #\1))
       (natp n)
       (< n (len inp)))
     (equal (val (take (+ 1 n) inp))
            (+ (* 2 (val (take n inp)))
               (if (eql (nth n inp) #\1) 1 0))))
   :enable (|take n+1| digit-count)
+  :disable |nth wordp is member|
   :use ((:instance |val append|
           (x (take n inp))
           (y (list (nth n inp))))
-        (:instance |nth word-01-p is member|
+        (:instance |nth wordp is member|
+          (alphabet '(#\0 #\1))
+          (x inp)
           (i n))))
 
 (defruled |step2 correct q|
   (implies
     (and
-      (word-01-p inp)
+      (wordp inp '(#\0 #\1))
       (natp n)
       (< n (len inp)))
     (simple-steps
@@ -515,28 +407,24 @@
      (defrule lemma2
        (implies
          (and
-           (word-01-p inp)
+           (wordp inp '(#\0 #\1))
            (natp n)
            (< n (len inp))
            (not (equal (nth n inp) #\1)))
          (equal (cons #\0 (replace-ones (nthcdr (+ 1 n) inp)))
                 (replace-ones (nthcdr n inp))))
-      :enable (|nthcdr as cons| replace-ones)
-      :use (:instance |nth word-01-p is member|
-             (i n)))
+      :enable (|nthcdr as cons| replace-ones))
      (defrule lemma3
        (implies
          (and
-           (word-01-p inp)
+           (wordp inp '(#\0 #\1))
            (natp n)
            (< n (len inp))
            (equal (nth n inp) #\1))
          (equal (list* #\0 #\| (replace-ones (nthcdr (+ 1 n) inp)))
                 (replace-ones (nthcdr n inp))))
-      :enable (|nthcdr as cons| replace-ones)
-      :use (:instance |nth word-01-p is member|
-             (i n))))
-  :enable (step2)
+      :enable (|nthcdr as cons| replace-ones)))
+  :enable (step2 |wordp replace-ones 0bar|)
   :use (:instance |step2 correct a|
          (i (val (take n inp)))
          (j (if (eql (nth n inp) #\1) 1 0))
@@ -545,7 +433,7 @@
 (defruled |step2 correct 4|
   (implies
     (and
-      (word-01-p inp)
+      (wordp inp '(#\0 #\1))
       (natp n)
       (<= n (len inp)))
     (simple-steps
@@ -558,7 +446,7 @@
     (defrule lemma
       (implies
         (and
-          (word-01-p inp)
+          (wordp inp '(#\0 #\1))
           (posp n)
           (<= n (len inp)))
         (equal
@@ -597,14 +485,14 @@
 |#
 (defruled |step2 0|
   (implies
-    (word-01-p inp)
+    (wordp inp '(#\0 #\1))
     (equal (step2 inp 0)
            (step1 inp (len inp))))
   :enable step2)
 
 (defruled |step2 len|
   (implies
-    (word-01-p inp)
+    (wordp inp '(#\0 #\1))
     (equal (step2 inp (len inp))
            (append (repeat (len inp) #\0)
                    (repeat (val inp) #\|))))
@@ -612,7 +500,7 @@
 
 (defruled |step1 and step2 correct|
   (implies
-    (word-01-p inp)
+    (wordp inp '(#\0 #\1))
     (simple-steps
       *scheme-bin2unary-ru*
       (val inp)
@@ -641,7 +529,7 @@
 (defruled |step3 applicable|
   (implies
     (and
-      (word-01-p inp)
+      (wordp inp '(#\0 #\1))
       (natp n)
       (< n (len inp)))
    (equal
@@ -671,7 +559,7 @@
 (defruled |step3 substp|
   (implies
     (and
-      (word-01-p inp)
+      (wordp inp '(#\0 #\1))
       (natp n)
       (< n (len inp)))
     (substp
@@ -695,7 +583,7 @@
 (defruled |step3 correct a|
   (implies
     (and
-      (word-01-p inp)
+      (wordp inp '(#\0 #\1))
       (natp n)
       (< n (len inp)))
     (simple-stepp
@@ -707,7 +595,7 @@
 (defruled |step3 correct b|
   (implies
     (and
-      (word-01-p inp)
+      (wordp inp '(#\0 #\1))
       (natp n)
       (<= n (len inp)))
     (simple-steps
@@ -728,21 +616,21 @@
 
 (defruled |step3 0|
   (implies
-    (word-01-p inp)
+    (wordp inp '(#\0 #\1))
     (equal (step3 inp 0)
            (step2 inp (len inp))))
   :enable (step3 |step2 len|))
 
 (defruled |step3 len|
   (implies
-    (word-01-p inp)
+    (wordp inp '(#\0 #\1))
     (equal (step3 inp (len inp))
            (repeat (val inp) #\|)))
   :enable step3)
 
 (defruled |step123 correct|
   (implies
-    (word-01-p inp)
+    (wordp inp '(#\0 #\1))
     (simple-steps
       *scheme-bin2unary-ru*
       (+ (val inp) (len inp))
